formalization/thys/Proof_Object.thy
@@ -1,67 +1,69 @@
+(*<*)
 theory Proof_Object
-imports Proof_System Partition
+  imports Formula Partition
 begin
+(*>*)
 
-subsection \<open>Proof Objects\<close>
+section \<open>Proof Objects\<close>
 
-datatype (dead 'd) sproof = STT nat 
-  | SPred nat Formula.name "'d Formula.trm list"
-  | SEq_Const nat Formula.name 'd
-  | SNeg "'d vproof" 
-  | SOrL "'d sproof" 
-  | SOrR "'d sproof" 
-  | SAnd "'d sproof" "'d sproof"
-  | SImpL "'d vproof" 
-  | SImpR "'d sproof"
-  | SIffSS "'d sproof" "'d sproof" 
-  | SIffVV "'d vproof" "'d vproof" 
-  | SExists Formula.name 'd "'d sproof"
-  | SForall Formula.name "('d, 'd sproof) part" 
-  | SPrev "'d sproof"
-  | SNext "'d sproof"
-  | SOnce nat "'d sproof"
-  | SEventually nat "'d sproof" 
-  | SHistorically nat nat "'d sproof list" 
+datatype (dead 'n, dead 'd) sproof = STT nat 
+  | SPred nat 'n "('n, 'd) Formula.trm list"
+  | SEq_Const nat 'n 'd
+  | SNeg "('n, 'd) vproof" 
+  | SOrL "('n, 'd) sproof" 
+  | SOrR "('n, 'd) sproof" 
+  | SAnd "('n, 'd) sproof" "('n, 'd) sproof"
+  | SImpL "('n, 'd) vproof" 
+  | SImpR "('n, 'd) sproof"
+  | SIffSS "('n, 'd) sproof" "('n, 'd) sproof" 
+  | SIffVV "('n, 'd) vproof" "('n, 'd) vproof" 
+  | SExists 'n 'd "('n, 'd) sproof"
+  | SForall 'n "('d, ('n, 'd) sproof) part" 
+  | SPrev "('n, 'd) sproof"
+  | SNext "('n, 'd) sproof"
+  | SOnce nat "('n, 'd) sproof"
+  | SEventually nat "('n, 'd) sproof" 
+  | SHistorically nat nat "('n, 'd) sproof list" 
   | SHistoricallyOut nat
-  | SAlways nat nat "'d sproof list"
-  | SSince "'d sproof" "'d sproof list" 
-  | SUntil "'d sproof list" "'d sproof" 
-  and 'd vproof = VFF nat 
-  | VPred nat Formula.name "'d Formula.trm list"
-  | VEq_Const nat Formula.name 'd
-  | VNeg "'d sproof" 
-  | VOr "'d vproof" "'d vproof"
-  | VAndL "'d vproof" 
-  | VAndR "'d vproof" 
-  | VImp "'d sproof" "'d vproof" 
-  | VIffSV "'d sproof" "'d vproof" 
-  | VIffVS "'d vproof" "'d sproof" 
-  | VExists Formula.name "('d, 'd vproof) part" 
-  | VForall Formula.name 'd "'d vproof"
-  | VPrev "'d vproof"
+  | SAlways nat nat "('n, 'd) sproof list"
+  | SSince "('n, 'd) sproof" "('n, 'd) sproof list" 
+  | SUntil "('n, 'd) sproof list" "('n, 'd) sproof" 
+  and ('n, 'd) vproof = VFF nat 
+  | VPred nat 'n "('n, 'd) Formula.trm list"
+  | VEq_Const nat 'n 'd
+  | VNeg "('n, 'd) sproof" 
+  | VOr "('n, 'd) vproof" "('n, 'd) vproof"
+  | VAndL "('n, 'd) vproof" 
+  | VAndR "('n, 'd) vproof" 
+  | VImp "('n, 'd) sproof" "('n, 'd) vproof" 
+  | VIffSV "('n, 'd) sproof" "('n, 'd) vproof" 
+  | VIffVS "('n, 'd) vproof" "('n, 'd) sproof" 
+  | VExists 'n "('d, ('n, 'd) vproof) part" 
+  | VForall 'n 'd "('n, 'd) vproof"
+  | VPrev "('n, 'd) vproof"
   | VPrevZ
   | VPrevOutL nat 
   | VPrevOutR nat
-  | VNext "'d vproof" 
+  | VNext "('n, 'd) vproof" 
   | VNextOutL nat 
   | VNextOutR nat 
   | VOnceOut nat 
-  | VOnce nat nat "'d vproof list" 
-  | VEventually nat nat "'d vproof list"
-  | VHistorically nat "'d vproof" 
-  | VAlways nat "'d vproof"
+  | VOnce nat nat "('n, 'd) vproof list" 
+  | VEventually nat nat "('n, 'd) vproof list"
+  | VHistorically nat "('n, 'd) vproof" 
+  | VAlways nat "('n, 'd) vproof"
   | VSinceOut nat
-  | VSince nat "'d vproof" "'d vproof list" 
-  | VSinceInf nat nat "'d vproof list" 
-  | VUntil nat "'d vproof list" "'d vproof"
-  | VUntilInf nat nat "'d vproof list"
+  | VSince nat "('n, 'd) vproof" "('n, 'd) vproof list" 
+  | VSinceInf nat nat "('n, 'd) vproof list" 
+  | VUntil nat "('n, 'd) vproof list" "('n, 'd) vproof"
+  | VUntilInf nat nat "('n, 'd) vproof list"
 
-type_synonym 'd "proof" = "'d sproof + 'd vproof"
+type_synonym ('n, 'd) "proof" = "('n, 'd) sproof + ('n, 'd) vproof"
 
-type_synonym 'd expl = "('d, 'd proof, Formula.name) pdt"
+type_synonym ('n, 'd) expl = "('d, ('n, 'd) proof, 'n) pdt"
 
-fun s_at :: "'d sproof \<Rightarrow> nat" and 
-  v_at :: "'d vproof \<Rightarrow> nat" where
+fun s_at :: "('n, 'd) sproof \<Rightarrow> nat" and 
+  v_at :: "('n, 'd) vproof \<Rightarrow> nat" where
   "s_at (STT i) = i"
 | "s_at (SPred i _ _) = i"
 | "s_at (SEq_Const i _ _) = i"
@@ -114,6 +116,8 @@ fun s_at :: "'d sproof \<Rightarrow> nat" and
 | "v_at (VUntil i _ _) = i"
 | "v_at (VUntilInf i _ _) = i"
 
-definition p_at :: "'d proof \<Rightarrow> nat" where "p_at p = case_sum s_at v_at p" 
+definition p_at :: "('n, 'd) proof \<Rightarrow> nat" where "p_at p = case_sum s_at v_at p" 
 
+(*<*)
 end
+(*>*)
